Add NonFaulty replicas with working examples

bft.v
@@ -8,29 +8,92 @@ Require Import String.
 Require Import Maps.
 Open Scope string_scope.
 
+
+Definition FNum := 2.
+Definition QuorumAcceptanceThreshold := 2*FNum + 1.
+Definition MaxMessages := 1000.
+
+
 Definition ReplicaId := string.
 Definition SysView := string.
 
 Inductive Message : Type := 
-| message: ReplicaId -> string -> Message.
+| reqMsg: string -> ReplicaId -> Message
+| pPrepMsg: string -> nat -> ReplicaId -> Message
+| prepMsg: string -> nat -> ReplicaId -> Message.
 
-Notation "<< rId , pLoad >>" := (message rId pLoad).
+Notation "<<REQ digest , rId >>" := (reqMsg digest rId).
+Notation "<<PPREP digest , seqNum , rId >>" := (pPrepMsg digest seqNum rId).
+Notation "<<PREP digest , seqNum , rId >>" := (prepMsg digest seqNum rId).
 
 
-Definition get_rId (msg : Message) : ReplicaId :=
+Definition GetRID (msg : Message) : ReplicaId :=
   match msg with
-  | message x y => x
+  | reqMsg digest rId => rId
+  | pPrepMsg digest seqNum rId => rId
+  | prepMsg digest seqNum rId => rId
   end.
 
-Definition get_pLoad (msg : Message) : string :=
+Definition GetDigest (msg : Message) : string :=
   match msg with
-  | message x y => y
+  | reqMsg digest rId => digest
+  | pPrepMsg digest seqNum rId => digest
+  | prepMsg digest seqNum rId => digest
   end.
 
-Definition Ledger := total_map nat.
+Definition Ledger := list (string * nat).
+Definition EmptyLedger : Ledger :=  nil.
+
+Fixpoint beq_ledgers (l1 l2 : Ledger) :=
+match l1 with
+| nil => match l2 with
+          | nil => true
+          | _ => false
+         end
+| (s1, n1)::t => match l2 with
+          | nil => false
+          | (s2, n2)::t2 => andb (andb (beq_string s1 s2) (beq_nat n1 n2)) (beq_ledgers t t2)
+         end
+end.
+
 Definition SysState := total_map Ledger.
 Definition MessageBox := list Message.
-Definition Replica := SysState -> Message -> MessageBox -> SysState.
+
+
+Inductive QCert : Type :=
+| qCert : string -> nat -> QCert.
+
+Definition QCerts := total_map (list QCert).
+
+Definition EmptyQCerts : QCerts := fun _ => nil.
+
+Inductive ExecEnvironment : Type :=
+| execEnv : list ReplicaId -> SysState -> QCerts -> MessageBox -> ExecEnvironment.
+
+
+Definition GetEnvState (env : ExecEnvironment) := 
+  match env with
+  | execEnv _ state _ _  => state
+  end.
+
+Definition GetEnvReplicas (env : ExecEnvironment) := 
+  match env with
+  | execEnv replicas _ _ _  => replicas
+  end.
+
+
+Definition GetEnvMsgBox (env : ExecEnvironment) := 
+  match env with
+  | execEnv _ _ _  mb => mb
+  end.
+
+Definition GetEnvQCerts (env : ExecEnvironment) := 
+  match env with
+  | execEnv _ _ qcs _ => qcs
+  end.
+
+Definition Replica := ExecEnvironment -> Message -> ExecEnvironment.
+
 Definition SysReplicas := list (ReplicaId * Replica).
 
 Inductive System : Type := 
@@ -45,6 +108,18 @@ Definition GetState (sys : System) :=
   match sys with
   | system _ state _ => state
   end.
+
+Fixpoint getReplicaIdsHelper (replicas : SysReplicas) (result : list ReplicaId) :=
+  match replicas with
+  | nil => result
+  | (rId, _)::t => rId::(getReplicaIdsHelper t result)
+  end.
+
+Definition GetReplicaIds (sys : System) := 
+  match sys with
+  | system _ _ replicas => (getReplicaIdsHelper replicas nil)
+  end.
+
 
 Definition GetReplicas (sys : System) := 
   match sys with
@@ -63,46 +138,125 @@ let replicas := GetReplicas sys in
   findReplicaHelper replicas rId.
 
 
-Definition empty_ledger : Ledger :=  (fun _ => 0).
-Definition empty_state : SysState :=  (fun _ => empty_ledger).
-Definition empty_replicas : SysReplicas :=  nil.
+Definition EmptyState : SysState :=  (fun _ => EmptyLedger).
+Definition EmptyReplicas : SysReplicas :=  nil.
 
-Definition ProcessMessage (sys:System) (rId : ReplicaId) (msg:Message) (msgBox : MessageBox) :=
- match (FindReplica sys rId) with
-    | None => sys
-    | Some replica =>
-      let sysState' := (replica (GetState sys) msg msgBox) in
-        (system "foo" sysState' (GetReplicas sys))
+Fixpoint multicast (from : ReplicaId) (replicas : list ReplicaId) (msgTo : ReplicaId -> Message) (mBox : MessageBox) : MessageBox :=
+  match replicas with
+  | nil => mBox
+  | rId::t => if (beq_string rId from) then multicast from t msgTo mBox
+              else (msgTo rId)::(multicast from t msgTo mBox)
   end.
 
-Fixpoint ProcessAllMessages (sys:System) (msgBox: MessageBox) : System := 
-  match msgBox with
-  | nil => sys
-  | msg::t => let rId := get_rId msg in
-              let sys' := ProcessMessage sys rId msg msgBox in
-                ProcessAllMessages sys' t
-  end
-.
+Definition pushCertificate (qCerts : QCerts) (rId : ReplicaId) (qCert : QCert) : QCerts :=
+  qCerts & {rId --> qCert::(qCerts rId)}.
 
-Definition Request := string.
+Fixpoint seqNumAccepted (l:Ledger) (n:nat) :=
+    match l with
+    | nil => false
+    | (_, v)::t => orb (beq_nat n v) (seqNumAccepted t n)
+    end.
 
-Definition ProcessRequest (sys : System) (req : Request) :=
-  ProcessAllMessages sys [<<"foo", req>>].
+Fixpoint hasEnoughQCerts (qCertL : list QCert) (digest : string) (seqNum collected : nat) :=
+    match qCertL with
+    | nil => beq_nat collected QuorumAcceptanceThreshold
+    | (qCert d v)::t => if (andb (beq_string digest d) (beq_nat v seqNum)) then
+                           hasEnoughQCerts t digest seqNum (S collected)
+                        else
+                            hasEnoughQCerts t digest seqNum collected
+    end.
 
+Definition isQuorumCertified (qCertsL : list QCert) (digest : string) (seqNum : nat):=
+    hasEnoughQCerts qCertsL digest seqNum 0.
+
+Definition pushSequenceNum (st : SysState) (rId : ReplicaId) (digest : string) (seqNum : nat) :=
+    st & {rId --> (digest, seqNum)::(st rId)}.
+
+Definition genSeqNum (l : Ledger) :=
+    match l with
+      | nil => 0
+      | (d, v)::t => S v
+    end.
+
+Definition NFReplica : Replica := 
+  fun env msg => 
+      match msg with
+      | (reqMsg digest rId) => let n := (genSeqNum ((GetEnvState env) rId)) in
+                                let mb' := (multicast rId (GetEnvReplicas env) (pPrepMsg digest n) (GetEnvMsgBox env)) in
+                                  let qCerts' := (pushCertificate (GetEnvQCerts env) rId (qCert digest n)) in
+                                    execEnv (GetEnvReplicas env) (GetEnvState env) qCerts' mb'
+      | (pPrepMsg digest n rId) => if (seqNumAccepted ((GetEnvState env) rId) n) then
+                                        env
+                                   else
+                                      let mb' := (multicast rId (GetEnvReplicas env) (prepMsg digest n) (GetEnvMsgBox env)) in
+                                      let qCerts' := (pushCertificate (GetEnvQCerts env) rId (qCert digest n)) in
+                                        if (isQuorumCertified (qCerts' rId) digest n) then
+                                           let state' := (pushSequenceNum (GetEnvState env) rId digest n) in
+                                              execEnv (GetEnvReplicas env) state' qCerts' mb'
+                                        else
+                                              execEnv (GetEnvReplicas env) (GetEnvState env) qCerts' mb'
+      | (prepMsg digest n rId) => if (seqNumAccepted ((GetEnvState env) rId) n) then
+                                        env
+                                   else
+                                      let qCerts' := (pushCertificate (GetEnvQCerts env) rId (qCert digest n)) in
+                                        if (isQuorumCertified (qCerts' rId) digest n) then
+                                           let state' := (pushSequenceNum (GetEnvState env) rId digest n) in
+                                              execEnv (GetEnvReplicas env) state' qCerts' (GetEnvMsgBox env)
+                                        else
+                                              execEnv (GetEnvReplicas env) (GetEnvState env) qCerts' (GetEnvMsgBox env)
+    end.
+
+Definition ProcessMessage (msg:Message) (sys:System) (rId : ReplicaId) (env : ExecEnvironment) :=
+ match (FindReplica sys rId) with
+    | None => env
+    | Some replica => (replica env msg)
+  end.
+
+Fixpoint ProcessAllMessages (fuel : nat) (sys:System) (env : ExecEnvironment) := 
+  match fuel with
+  | 0 => env
+  | S f' =>
+      match (GetEnvMsgBox env) with
+      | nil => env
+      | msg::t => let rId := GetRID msg in
+                  let envI := (execEnv (GetEnvReplicas env) (GetEnvState env) (GetEnvQCerts env) t) in
+                  let env' := ProcessMessage msg sys rId envI in
+                    ProcessAllMessages f' sys env'
+      end
+  end.
+
+Print ExecEnvironment.
+Print System.
+Definition ProcessRequest (sys : System) (req : Message) : System :=
+  let env' := ProcessAllMessages MaxMessages sys (execEnv (GetReplicaIds sys) (GetState sys) EmptyQCerts [req]) in
+    (system "" (GetEnvState env') (GetReplicas sys)).
+
+Fixpoint getCommonLedger (state : SysState) (replicas: SysReplicas) (gLedger : Ledger) :=
+match replicas with
+    | nil => Some gLedger
+    | (rId, _)::t => if (beq_ledgers (state rId) gLedger) then (getCommonLedger state t gLedger)
+                      else None
+end.
+
+Definition GetGlobalLedger (sys:System) : option Ledger :=
+  let state := GetState sys in
+    let gLedger := state "primary" in
+      let replicas := GetReplicas sys in
+         getCommonLedger state replicas gLedger.
+(*
 Definition NonFaulty (rId : ReplicaId) : Prop := True.
 Definition MajorityNonFaulty (sys:System) : Prop := True.
 
 Inductive StateValid : System -> Prop :=
-| empty_valid : forall sys:System, (GetState sys) = empty_state 
+| empty_valid : forall sys:System, (GetState sys) = EmptyState 
                   -> StateValid sys.
 
 
-Lemma system_safety: forall (sys:System) (msgBox:MessageBox),
+Lemma system_safety: forall (sys:System),
   MajorityNonFaulty sys
-  -> StateValid (ProcessAllMessages sys msgBox)
-  -> forall (m:Message), StateValid (ProcessAllMessages sys (m::msgBox)).
+  -> StateValid sys
+  -> forall (r:Request), StateValid (ProcessRequest sys r).
 Proof. Admitted.
-
 
 Theorem byzantine_fault_tolerant : forall (sys:System) (msgBox : MessageBox),
     MajorityNonFaulty sys 
@@ -114,5 +268,5 @@ induction msgBox.
   - induction replicas.
     + apply IHmsgBox.
     + apply system_safety; assumption.
-Qed.
+Qed.*)
 
