example-tests.v
@@ -3,39 +3,54 @@ Require Import Maps.
 Require Import Coq.Lists.List.
 Import ListNotations.
 
-Definition one_replicas : SysReplicas := ("foo", fun _ _ _ => empty_state)::empty_replicas.
-Definition system1 := (system "foo" empty_state one_replicas).
-Definition m1 := <<"foo", "1">>.
+Definition replicas1 : SysReplicas := ("foo", fun env _ => env)::EmptyReplicas.
+Definition system1 := (system "foo" EmptyState replicas1).
+Definition m1 := <<REQ "foo", "1">>.
 Definition twoMsgBox := [m1 ; m1].
+Print ExecEnvironment.
+Definition execEnv1 := (execEnv (GetReplicaIds system1) EmptyState EmptyQCerts nil).
 
-Example sysEmptyTest : GetState (ProcessAllMessages system1 twoMsgBox) = empty_state.
+Example sysEmptyTest : GetEnvState (ProcessAllMessages MaxMessages system1 execEnv1) = EmptyState.
 Proof. reflexivity. Qed.
 
-Example stValid_ProcMessages_sys1 : StateValid (ProcessAllMessages system1 twoMsgBox).
-Proof. constructor. reflexivity.   Qed.
+Definition activeReplicas1 : SysReplicas :=  
+      ("foo" , NFReplica )
+      ::EmptyReplicas.
+Definition activeSystem1 := (system "" EmptyState activeReplicas1).
+Definition activeEnv1 := (execEnv (GetReplicaIds activeSystem1) (EmptyState) EmptyQCerts [<<REQ "1", "foo"  >> ]).
 
-Print Replica.
-Print Ledger.
+Compute (GetEnvState (ProcessAllMessages MaxMessages activeSystem1 activeEnv1)) "foo".
+Example activeSystem1_noState : (GetEnvState (ProcessAllMessages MaxMessages activeSystem1 activeEnv1)) = EmptyState.
+Proof. reflexivity. Qed.
 
-Definition active_replicas : SysReplicas :=  
-      ("foo" , fun sysSt msg mb => sysSt & {"foo" --> (empty_ledger & { (get_pLoad msg) --> 1 }) } )
-      ::empty_replicas.
-Definition systemActive := (system "foo" empty_state active_replicas).
-Example stValid_ProcMessages_sysActive : StateValid (ProcessAllMessages systemActive twoMsgBox).
-Proof.  repeat apply system_safety; constructor; reflexivity.
+Compute (GetEnvQCerts (ProcessAllMessages MaxMessages activeSystem1 activeEnv1)) "foo".
+Example activeSystem1_oneCertificate : length ((GetEnvQCerts (ProcessAllMessages MaxMessages activeSystem1 activeEnv1)) "foo") = 1.
+Proof. reflexivity. Qed.
+
+Compute (GetEnvMsgBox (ProcessAllMessages MaxMessages activeSystem1 activeEnv1)).
+Example activeSystem1_emptyMessages : length (GetEnvMsgBox (ProcessAllMessages MaxMessages activeSystem1 activeEnv1)) = 0.
+Proof. reflexivity. Qed.
+
+Definition multipleActiveReplicas : SysReplicas :=
+      ("foo" , NFReplica )::("foo1" , NFReplica )::("foo2" , NFReplica )::("primary" , NFReplica )::("foo4" , NFReplica )
+      ::("foo5" , NFReplica )::("foo6" , NFReplica )::("foo7" , NFReplica )
+      ::("foo9" , NFReplica )::("foo8" , NFReplica )::EmptyReplicas.
+
+Definition multiReplicaSys := (system "" EmptyState multipleActiveReplicas).
+Definition multiReplicaEnv := (execEnv (GetReplicaIds multiReplicaSys) (EmptyState) EmptyQCerts [<<REQ "digest", "primary" >>]).
+
+Compute (GetEnvState (ProcessAllMessages MaxMessages multiReplicaSys multiReplicaEnv)) "foo5".
+Compute (GetState (ProcessRequest multiReplicaSys <<REQ "digest", "primary" >>)) "foo".
+
+Example procRequest_multiReplicaSys : (GetState (ProcessRequest multiReplicaSys <<REQ "digest", "primary" >>) ) "primary" = [("digest", 0)].
+Proof. reflexivity. Qed.
+
+Definition processedSys := ProcessRequest multiReplicaSys <<REQ "digest", "primary" >>.
+
+Example globalLedgerConsistent : let sys' := (ProcessRequest multiReplicaSys <<REQ "digest", "primary" >>) in 
+                                  GetGlobalLedger sys' =  Some ((GetState sys') "primary").
+Proof. intros. reflexivity. 
 Qed.
 
-Definition multiple_active_replicas : SysReplicas :=
-      ("foo" , fun sysSt msg mb => sysSt & {"foo" --> (empty_ledger & { (get_pLoad msg) --> 1 }) } )
-      :: ("bar" , fun sysSt msg mb => sysSt & {"bar" --> (empty_ledger & { (get_pLoad msg) --> 1 }) } )
-      :: ("baz" , fun sysSt msg mb => sysSt & {"baz" --> (empty_ledger & { (get_pLoad msg) --> 1 }) } )
-      ::empty_replicas.
-
-Definition multi_replica_sys := (system "" empty_state multiple_active_replicas).
-Definition multi_replica_msgBox := [<<"foo", "1">> ; <<"bar" , "1">>; <<"baz" , "1">>].
-
-Example stValid_ProcMessages_multi_replicas : StateValid (ProcessAllMessages multi_replica_sys multi_replica_msgBox).
-Proof.  repeat apply system_safety; constructor; reflexivity.
-Qed.
 
 
